src/Distributions/UniformPowerOfTwo/Model.dfy
@@ -7,13 +7,13 @@ module UniformPowerOfTwo.Model {
   import Helper
   import Rand
   import Quantifier
-  import Monad
+  import Monad`Spec
 
   // Adapted from Definition 48 (see issue #79 for the reason of the modification)
   // The return value u is uniformly distributed between 0 <= u < 2^k where 2^k <= n < 2^(k + 1).
   opaque function Sample(n: nat): (h: Monad.Hurd<nat>)
     requires n >= 1
-    ensures forall s :: Sample(n)(s).Result? // always terminates, not just almost surely
+    //ensures forall s :: Sample(n)(s).Result? // always terminates, not just almost surely
   {
     if n == 1 then
       Monad.Return(0)
@@ -26,6 +26,6 @@ module UniformPowerOfTwo.Model {
   }
 
   function UnifStep(m: nat): Monad.Hurd<nat> {
-    Monad.Bind(Monad.Coin, UnifStepHelper(m))
+    Monad.Bind(Monad.Coin(), UnifStepHelper(m))
   }
 }
